Source/DafnyCore/Resolver/PreType/PreTypeResolve.cs
@@ -177,7 +177,7 @@ namespace Microsoft.Dafny {
       Contract.Requires(type != null);
 
       type = type.Normalize(); // keep type synonyms
-      if (type.AsTypeSynonym is { } typeSynonymDecl and not SubsetTypeDecl && option != Type2PreTypeOption.GoodForInference &&
+      if (type.AsTypeSynonym is { } typeSynonymDecl && option != Type2PreTypeOption.GoodForInference &&
           typeSynonymDecl.IsRevealedInScope(Type.GetScope())) {
         // Compute a pre-type for the non-instantiated ("raw") RHS type (that is, for the RHS of the type-synonym declaration with the
         // formal type parameters of the type-synonym declaration).
@@ -224,7 +224,7 @@ namespace Microsoft.Dafny {
       return new DPreType(decl, arguments);
     }
 
-    TopLevelDecl Type2Decl(Type type) {
+    public TopLevelDecl Type2Decl(Type type) {
       Contract.Requires(type != null);
       Contract.Requires(type is NonProxyType and not SelfType);
       TopLevelDecl decl;
