Test/dafny2/pq-intrinsic-extrinsic.dfy
@@ -1,4 +1,4 @@
-// RUN: %testDafnyForEachCompiler "%s" -- --relax-definite-assignment
+// RUN: %testDafnyForEachCompiler --refresh-exit-code=0 "%s" -- --relax-definite-assignment
 
 // This file contains several versions of a priority queue implemented by Braun trees:
 //
